Merge with James' hounours work 1/x: fix semantics/proofs
Co-authored-by: James Shaker <james.shaker@gmail.com>

semantics/payloadSemScript.sml
@@ -8,106 +8,115 @@ val _ = Datatype `
        | LTau
 `
 
-val (trans_rules,trans_ind,trans_cases) = Hol_reln `
-
+Inductive trans:
   (* Send-last-payload *)
   (∀conf s v n d p1 p2 e.
     FLOOKUP s.bindings v = SOME d
     ∧ LENGTH d - n <= conf.payload_size
     ∧ p1 ≠ p2
-    ⇒ trans conf (NEndpoint p1 s (Send p2 v n e)) (LSend p1 (pad conf (DROP n d)) p2) (NEndpoint p1 s e))
+    ⇒ trans conf (NEndpoint p1 s (Send p2 v n e))
+                 (LSend p1 (pad conf (DROP n d)) p2)
+                 (NEndpoint p1 s e)) ∧
 
   (* Send-intermediate-payload *)
-∧ (∀conf s v n d p1 p2 e.
+  (∀conf s v n d p1 p2 e.
     FLOOKUP s.bindings v = SOME d
     ∧ LENGTH d - n > conf.payload_size
     ∧ p1 ≠ p2
     ⇒ trans conf (NEndpoint p1 s (Send p2 v n e))
                   (LSend p1 (pad conf (DROP n d)) p2)
-                  (NEndpoint p1 s (Send p2 v (n + conf.payload_size) e)))
+                  (NEndpoint p1 s (Send p2 v (n + conf.payload_size) e))) ∧
 
   (* Enqueue *)
-∧ (∀conf s d p1 p2 e.
+  (∀conf s d p1 p2 e.
     p1 ≠ p2
     ⇒ trans conf (NEndpoint p2 s e)
              (LReceive p1 d p2)
-             (NEndpoint p2 (s with queue := SNOC (p1,d) s.queue) e))
+             (NEndpoint p2 (s with queues := qpush s.queues p1 d) e)) ∧
 
   (* Com-L *)
-∧ (∀conf n1 n2 p1 p2 d n1' n2'.
+  (∀conf n1 n2 p1 p2 d n1' n2'.
     p1 ≠ p2
     ∧ trans conf n1 (LSend p1 d p2) n1'
     ∧ trans conf n2 (LReceive p1 d p2) n2'
-    ⇒ trans conf (NPar n1 n2) LTau (NPar n1' n2'))
+    ⇒ trans conf (NPar n1 n2) LTau (NPar n1' n2')) ∧
 
   (* Com-R *)
-∧ (∀conf n1 n2 p1 p2 d n1' n2'.
+  (∀conf n1 n2 p1 p2 d n1' n2'.
     p1 ≠ p2
     ∧ trans conf n1 (LReceive p1 d p2) n1'
     ∧ trans conf n2 (LSend p1 d p2) n2'
-    ⇒ trans conf (NPar n1 n2) LTau (NPar n1' n2'))
+    ⇒ trans conf (NPar n1 n2) LTau (NPar n1' n2')) ∧
 
   (* Dequeue-last-payload *)
-∧ (∀conf s v p1 p2 e q1 q2 d ds.
-    s.queue = q1 ++ [(p1,d)] ++ q2
-    ∧ p1 ≠ p2
-    ∧ EVERY (λ(p,_). p ≠ p1) q1
+  (∀conf s v p1 p2 e d tl ds.
+    p1 ≠ p2
+    ∧ qlk s.queues p1 = d::tl
     ∧ final d
     ⇒ trans conf (NEndpoint p2 s (Receive p1 v ds e))
              LTau
-             (NEndpoint p2 (s with <|queue := q1 ++ q2;
-                                     bindings := s.bindings |+ (v,FLAT(SNOC (unpad d) ds))|>) e))
+             (NEndpoint p2
+                        (s with <|queues :=
+                                    s.queues   |+ (p1,tl);
+                                  bindings :=
+                                    s.bindings |+ (v,FLAT(SNOC (unpad d) ds))
+                                  |>)
+                        e)) ∧
 
   (* Dequeue-intermediate-payload *)
-∧ (∀conf s v p1 p2 e q1 q2 d ds.
-    s.queue = q1 ++ [(p1,d)] ++ q2
-    ∧ p1 ≠ p2
-    ∧ EVERY (λ(p,_). p ≠ p1) q1
+  (∀conf s v p1 p2 e d tl ds.
+    p1 ≠ p2
+    ∧ qlk s.queues p1 = d::tl
     ∧ intermediate d
     ⇒ trans conf (NEndpoint p2 s (Receive p1 v ds e))
              LTau
-             (NEndpoint p2 (s with queue := q1 ++ q2) (Receive p1 v (SNOC (unpad d) ds) e)))
+             (NEndpoint p2 (s with queues :=
+                                    s.queues |+ (p1,tl))
+                           (Receive p1 v (SNOC (unpad d) ds) e))) ∧
 
   (* If-L *)
-∧ (∀conf s v p e1 e2.
+  (∀conf s v p e1 e2.
     FLOOKUP s.bindings v = SOME [1w]
     ⇒ trans conf (NEndpoint p s (IfThen v e1 e2))
              LTau
-             (NEndpoint p s e1))
+             (NEndpoint p s e1)) ∧
 
   (* If-R *)
-∧ (∀conf s v p e1 e2 w.
+  (∀conf s v p e1 e2 w.
     FLOOKUP s.bindings v = SOME w ∧ w ≠ [1w]
     ⇒ trans conf (NEndpoint p s (IfThen v e1 e2))
              LTau
-             (NEndpoint p s e2))
+             (NEndpoint p s e2)) ∧
 
   (* Let *)
-∧ (∀conf s v p f vl e.
+  (∀conf s v p f vl e.
     EVERY IS_SOME (MAP (FLOOKUP s.bindings) vl)
     ⇒ trans conf (NEndpoint p s (Let v f vl e))
              LTau
-             (NEndpoint p (s with bindings := s.bindings |+ (v,f(MAP (THE o FLOOKUP s.bindings) vl))) e))
+             (NEndpoint p
+                        (s with bindings :=
+                          s.bindings |+ (v,f(MAP (THE o FLOOKUP s.bindings) vl)))
+                        e)) ∧
 
   (* Par-L *)
-∧ (∀conf n1 n1' n2 alpha.
-    trans conf n1 alpha n1'
+  (∀conf n1 n1' n2 α.
+    trans conf n1 α n1'
     ⇒ trans conf (NPar n1 n2)
-             alpha
-             (NPar n1' n2))
+             α
+             (NPar n1' n2)) ∧
 
   (* Par-R *)
-∧ (∀conf n1 n2 n2' alpha.
-    trans conf n2 alpha n2'
+  (∀conf n1 n2 n2' α.
+    trans conf n2 α n2'
     ⇒ trans conf (NPar n1 n2)
-             alpha
+             α
              (NPar n1 n2'))
-`
+End
 
- val _ = zip ["trans_send_last_payload","trans_send_intermediate_payload",
-              "trans_enqueue","trans_com_l","trans_com_r",
-              "trans_dequeue_last_payload","trans_dequeue_intermediate_payload",
-              "trans_if_true","trans_if_false","trans_let","trans_par_l","trans_par_r"]
+val _ = zip ["trans_send_last_payload","trans_send_intermediate_payload",
+             "trans_enqueue","trans_com_l","trans_com_r",
+             "trans_dequeue_last_payload","trans_dequeue_intermediate_payload",
+             "trans_if_true","trans_if_false","trans_let","trans_par_l","trans_par_r"]
             (CONJUNCTS trans_rules) |> map save_thm;
 
 val reduction_def = Define `
