semantics/proofs/payloadPropsScript.sml
@@ -48,450 +48,69 @@ val endpoints_def = Define `
 /\ (endpoints (NEndpoint p1 s e1) = [(p1,s,e1)])
 /\ (endpoints (NPar n1 n2) = endpoints n1 ++ endpoints n2)`
 
-val (qcong_rules, qcong_ind, qcong_cases) = Hol_reln `
-  (* Reflexive *)
-  (∀n. qcong n n)
-
-  (* Symmetric *)
-∧ (∀n1 n2.
-    qcong n1 n2
-    ⇒ qcong n2 n1)
-  (* Transitive *)
-∧ (∀n1 n2 n3.
-     qcong n1 n2
-     ∧ qcong n2 n3
-     ⇒ qcong n1 n3)
-
-  (* Queue-Reorder *)
-∧ (∀p s e p1 d1 p2 d2 q1 q2.
-    s.queue = q1 ++ [(p1,d1);(p2,d2)] ++ q2
-    ∧ p1 ≠ p2
-    ⇒ qcong (NEndpoint p s e) (NEndpoint p (s with queue:= q1 ++ [(p2,d2);(p1,d1)] ++ q2) e))
-
-  (* Par *)
-∧ (∀n1 n2 n3 n4.
-     qcong n1 n2
-     ∧ qcong n3 n4
-     ⇒ qcong (NPar n1 n3) (NPar n2 n4))`
-
-val [qcong_refl,qcong_sym,qcong_trans,qcong_queue_reorder,qcong_par]
-    = zip ["qcong_refl","qcong_sym","qcong_trans","qcong_queue_reorder","qcong_par"]
-          (CONJUNCTS qcong_rules) |> map save_thm;
-
-val qcong_strongind = fetch "-" "qcong_strongind"
-
-val (qrel_rules, qrel_ind, qrel_cases) = Hol_reln `
-  (* Reflexive *)
-  (∀q. qrel q q)
-
-  (* Symmetric *)
-∧ (∀q1 q2.
-    qrel q1 q2
-    ⇒ qrel q2 q1)
-  (* Transitive *)
-∧ (∀q1 q2 q3.
-     qrel q1 q2
-     ∧ qrel q2 q3
-     ⇒ qrel q1 q3)
-
-  (* Queue-Reorder *)
-∧ (∀p1 d1 p2 d2 q1 q2.
-    p1 ≠ p2
-    ⇒ qrel (q1 ++ [(p1,d1);(p2,d2)] ++ q2) (q1 ++ [(p2,d2);(p1,d1)] ++ q2))`
-
-val qrel_strongind = fetch "-" "qrel_strongind"
-
-val [qrel_refl,qrel_sym,qrel_trans,qrel_queue_reorder]
-    = zip ["qrel_refl","qrel_sym","qrel_trans","qrel_queue_reorder"]
-          (CONJUNCTS qrel_rules) |> map save_thm;
-
-val qcong_queue_reorder' = Q.store_thm("qcong_queue_reorder'",
-  `∀p s e p1 d1 p2 d2 q1 q2.
-     p1 ≠ p2
-     ⇒ qcong (NEndpoint p (s with queue:=q1 ++ [(p1,d1);(p2,d2)] ++ q2) e)
-              (NEndpoint p (s with queue:= q1 ++ [(p2,d2);(p1,d1)] ++ q2) e)`,
-  rpt strip_tac
-  >> qmatch_goalsub_abbrev_tac `qcong (NEndpoint _ (_ with queue := a1) _) (NEndpoint _ (_ with queue := a2) _)`
-  >> `s with queue := a2 = (s with queue := a1) with queue := a2` by fs[]
-  >> pop_assum (fn thm => PURE_ONCE_REWRITE_TAC [thm])
-  >> unabbrev_all_tac
-  >> match_mp_tac qcong_queue_reorder
-  >> simp[]);
-
-val qrel_IMP_qcong = Q.store_thm("qrel_IMP_qcong",
-  `!q1 q2 p s e.
-    qrel q1 q2
-    ==> qcong (NEndpoint p (s with queue := q1) e) (NEndpoint p (s with queue := q2) e)`,
-  simp[GSYM PULL_FORALL]
-  >> ho_match_mp_tac qrel_strongind
-  >> metis_tac[qcong_rules,qcong_queue_reorder'])
-
-val qrel_cons = Q.store_thm("qrel_cons",
-  `!q1 q2 qe. qrel q1 q2 ==> qrel (qe::q1) (qe::q2)`,
-  simp[GSYM AND_IMP_INTRO,GSYM PULL_FORALL]
-  >> ho_match_mp_tac qrel_strongind >> rpt strip_tac
-  >- metis_tac[qrel_rules]
-  >- metis_tac[qrel_rules]
-  >- metis_tac[qrel_rules]
-  >> `!a b. qe::(a ++ b) = qe::a ++ b` by simp[]
-  >> ASM_SIMP_TAC pure_ss [] >> pop_assum kall_tac
-  >> metis_tac[qrel_rules]);
-
-val qrel_snoc = Q.store_thm("qrel_snoc",
-  `!q1 q2 qe. qrel q1 q2 ==> qrel (SNOC qe q1) (SNOC qe q2)`,
-  simp[GSYM AND_IMP_INTRO,GSYM PULL_FORALL]
-  >> ho_match_mp_tac qrel_strongind >> rpt strip_tac
-  >- metis_tac[qrel_rules]
-  >- metis_tac[qrel_rules]
-  >- metis_tac[qrel_rules]
-  >> simp[SNOC_APPEND]
-  >> metis_tac[qrel_rules,APPEND_ASSOC]);
-
-val qrel_append_l = Q.store_thm("qrel_append_l",
-  `!q1 q2 q3. qrel q2 q3 ==> qrel (q1++q2) (q1++q3)`,
-  Induct >> simp[] >> metis_tac[qrel_cons]);
-
-val qrel_append_r = Q.store_thm("qrel_append_r",
-  `!q3 q1 q2. qrel q1 q2 ==> qrel (q1++q3) (q2++q3)`,
-  ho_match_mp_tac SNOC_INDUCT >> rpt strip_tac >> simp[APPEND_SNOC] >> metis_tac[qrel_snoc]);
-
-val qrel_append = Q.store_thm("qrel_append",
-  `!q1 q2 q3 q4. qrel q1 q2 /\ qrel q3 q4 ==> qrel (q1++q3) (q2++q4)`,
-  metis_tac[qrel_rules,qrel_append_l,qrel_append_r]);
-
-val qrel_LENGTH = Q.store_thm("qrel_LENGTH",
-  `!q1 q2. qrel q1 q2 ==> LENGTH q1 = LENGTH q2`,
-  ho_match_mp_tac qrel_ind >> rw[]);
-
-val qrel_PERM = Q.store_thm("qrel_PERM",
-  `!q1 q2. qrel q1 q2 ==> PERM q1 q2`,
-  ho_match_mp_tac qrel_strongind
-  >> rpt strip_tac
-  >> fs[PERM_SYM]
-  >- metis_tac[PERM_TRANS]
-  >- CONV_TAC permLib.PERM_ELIM_DUPLICATES_CONV);
-
-val qrel_cons_IMP_lemma = Q.prove(
-  `!q1l q1r q2 qe. qrel (q1l ++ [qe] ++ q1r) q2 /\ EVERY (λ(p,_). p ≠ FST qe) q1l ==> ?q2l q2r. q2 = q2l ++ [qe] ++ q2r /\ qrel (q1l ++ q1r) (q2l++q2r) /\ EVERY (λ(p,_). p ≠ FST qe) q2l`,
-  `!q1 q2. qrel q1 q2 ==> ((!q1l q1r qe. q1 = q1l ++ [qe] ++ q1r /\ EVERY (λ(p,_). p ≠ FST qe) q1l ==> ?q2l q2r. q2 = q2l ++ [qe] ++ q2r /\ qrel (q1l++q1r) (q2l++q2r) /\ EVERY (λ(p,_). p ≠ FST qe) q2l)
-                           /\ (!q2l q2r qe. q2 = q2l ++ [qe] ++ q2r /\ EVERY (λ(p,_). p ≠ FST qe) q2l ==> ?q1l q1r. q1 = q1l ++ [qe] ++ q1r /\ qrel (q1l++q1r) (q2l++q2r) /\ EVERY (λ(p,_). p ≠ FST qe) q1l))`
-    suffices_by metis_tac[]
-  >> ho_match_mp_tac qrel_strongind >> rpt strip_tac >> rveq
-  >- metis_tac[qrel_refl]
-  >- metis_tac[qrel_refl]
-  >- metis_tac[qrel_sym]
-  >- metis_tac[qrel_sym]
-  >- (last_x_assum (qspecl_then [`q1l`,`q1r`,`qe`] assume_tac)
-      >> rfs[] >> rveq
-      >> last_x_assum (qspecl_then [`q2l`,`q2r`,`qe`] assume_tac)
-      >> rfs[] >> rveq
-      >> last_x_assum (qspecl_then [`q2l`,`q2r`,`qe`] assume_tac)
-      >> rfs[] >> rveq
-      >> last_x_assum (qspecl_then [`q2l'`,`q2r'`,`qe`] assume_tac) (* TODO: generated names *)
-      >> rfs[] >> rveq
-      >> metis_tac[qrel_trans])
-  >- (first_x_assum (qspecl_then [`q2l`,`q2r`,`qe`] assume_tac)
-      >> rfs[] >> rveq
-      >> first_x_assum (qspecl_then [`q1l`,`q1r`,`qe`] assume_tac)
-      >> rfs[] >> rveq
-      >> first_x_assum (qspecl_then [`q1l`,`q1r`,`qe`] assume_tac)
-      >> rfs[] >> rveq
-      >> first_x_assum (qspecl_then [`q1l'`,`q1r'`,`qe`] assume_tac) (* TODO: generated names *)
-      >> rfs[] >> rveq
-      >> metis_tac[qrel_trans])
-  >- (qpat_x_assum `_ = _` (assume_tac o REWRITE_RULE [APPEND_EQ_APPEND_MID |> CONV_RULE(LHS_CONV SYM_CONV)])
-      >> fs[] >> rveq
-      >- (qexists_tac `q1l` >> rw[]
-          >> metis_tac[qrel_queue_reorder,APPEND_ASSOC])
-      >- (rename1 `[_;_] = a1 ++ _ ++ _`
-          >> Cases_on `a1`
-          >- (fs[] >> rveq >> qexists_tac `q1++[(p2,d2)]` >> rw[qrel_refl])
-          >> fs[] >> rveq
-          >> fs[APPEND_EQ_SING |> CONV_RULE(LHS_CONV SYM_CONV)] >> rveq
-          >> qexists_tac `q1` >> rw[]
-          >> qmatch_goalsub_abbrev_tac `qrel a1 a2`
-          >> `a1 = a2` suffices_by rw[qrel_refl]
-          >> unabbrev_all_tac
-          >> rw[])
-      >- (qexists_tac `q1 ++ [(p2,d2); (p1,d1)] ++ l` >> rw[] >> fs[EVERY_APPEND]
-          >> metis_tac[qrel_queue_reorder,APPEND_ASSOC]))
-  >- (qpat_x_assum `_ = _` (assume_tac o REWRITE_RULE [APPEND_EQ_APPEND_MID |> CONV_RULE(LHS_CONV SYM_CONV)])
-      >> fs[] >> rveq
-      >- (qexists_tac `q2l` >> rw[]
-          >> metis_tac[qrel_queue_reorder,APPEND_ASSOC])
-      >- (rename1 `[_;_] = a1 ++ _ ++ _`
-          >> Cases_on `a1`
-          >- (fs[] >> rveq >> qexists_tac `q1++[(p1,d1)]` >> rw[qrel_refl])
-          >> fs[] >> rveq
-          >> fs[APPEND_EQ_SING |> CONV_RULE(LHS_CONV SYM_CONV)] >> rveq
-          >> qexists_tac `q1` >> rw[]
-          >> qmatch_goalsub_abbrev_tac `qrel a1 a2`
-          >> `a1 = a2` suffices_by rw[qrel_refl]
-          >> unabbrev_all_tac
-          >> rw[])
-      >- (qexists_tac `q1 ++ [(p1,d1); (p2,d2)] ++ l` >> rw[] >> fs[EVERY_APPEND]
-          >> metis_tac[qrel_queue_reorder,APPEND_ASSOC])));
-
-val qrel_snoc_IMP_lemma = Q.prove(
-  `!q1l q1r q2 qe. qrel (q1l ++ [qe] ++ q1r) q2 /\ EVERY (λ(p,_). p ≠ FST qe) q1r ==> ?q2l q2r. q2 = q2l ++ [qe] ++ q2r /\ qrel (q1l ++ q1r) (q2l++q2r) /\ EVERY (λ(p,_). p ≠ FST qe) q2r`,
-  `!q1 q2. qrel q1 q2 ==> ((!q1l q1r qe. q1 = q1l ++ [qe] ++ q1r /\ EVERY (λ(p,_). p ≠ FST qe) q1r ==> ?q2l q2r. q2 = q2l ++ [qe] ++ q2r /\ qrel (q1l++q1r) (q2l++q2r) /\ EVERY (λ(p,_). p ≠ FST qe) q2r)
-                           /\ (!q2l q2r qe. q2 = q2l ++ [qe] ++ q2r /\ EVERY (λ(p,_). p ≠ FST qe) q2r ==> ?q1l q1r. q1 = q1l ++ [qe] ++ q1r /\ qrel (q1l++q1r) (q2l++q2r) /\ EVERY (λ(p,_). p ≠ FST qe) q1r))`
-    suffices_by metis_tac[]
-  >> ho_match_mp_tac qrel_strongind >> rpt strip_tac >> rveq
-  >- metis_tac[qrel_refl]
-  >- metis_tac[qrel_refl]
-  >- metis_tac[qrel_sym]
-  >- metis_tac[qrel_sym]
-  >- (last_x_assum (qspecl_then [`q1l`,`q1r`,`qe`] assume_tac)
-      >> rfs[] >> rveq
-      >> last_x_assum (qspecl_then [`q2l`,`q2r`,`qe`] assume_tac)
-      >> rfs[] >> rveq
-      >> last_x_assum (qspecl_then [`q2l`,`q2r`,`qe`] assume_tac)
-      >> rfs[] >> rveq
-      >> last_x_assum (qspecl_then [`q2l'`,`q2r'`,`qe`] assume_tac) (* TODO: generated names *)
-      >> rfs[] >> rveq
-      >> metis_tac[qrel_trans])
-  >- (first_x_assum (qspecl_then [`q2l`,`q2r`,`qe`] assume_tac)
-      >> rfs[] >> rveq
-      >> first_x_assum (qspecl_then [`q1l`,`q1r`,`qe`] assume_tac)
-      >> rfs[] >> rveq
-      >> first_x_assum (qspecl_then [`q1l`,`q1r`,`qe`] assume_tac)
-      >> rfs[] >> rveq
-      >> first_x_assum (qspecl_then [`q1l'`,`q1r'`,`qe`] assume_tac) (* TODO: generated names *)
-      >> rfs[] >> rveq
-      >> metis_tac[qrel_trans])
-  >- (qpat_x_assum `_ = _` (assume_tac o REWRITE_RULE [APPEND_EQ_APPEND_MID |> CONV_RULE(LHS_CONV SYM_CONV)])
-      >> fs[] >> rveq
-      >- (qexists_tac `q1l` >> rw[] >> fs[EVERY_APPEND]
-          >> metis_tac[qrel_queue_reorder,APPEND_ASSOC,EVERY_APPEND])
-      >- (rename1 `[_;_] = a1 ++ _ ++ _`
-          >> Cases_on `a1`
-          >- (fs[] >> rveq >> qexists_tac `q1++[(p2,d2)]` >> rw[qrel_refl])
-          >> fs[] >> rveq
-          >> fs[APPEND_EQ_SING |> CONV_RULE(LHS_CONV SYM_CONV)] >> rveq
-          >> qexists_tac `q1` >> rw[]
-          >> qmatch_goalsub_abbrev_tac `qrel a1 a2`
-          >> `a1 = a2` suffices_by rw[qrel_refl]
-          >> unabbrev_all_tac
-          >> rw[])
-      >- (qexists_tac `q1 ++ [(p2,d2); (p1,d1)] ++ l` >> rw[] >> fs[EVERY_APPEND]
-          >> metis_tac[qrel_queue_reorder,APPEND_ASSOC]))
-  >- (qpat_x_assum `_ = _` (assume_tac o REWRITE_RULE [APPEND_EQ_APPEND_MID |> CONV_RULE(LHS_CONV SYM_CONV)])
-      >> fs[] >> rveq
-      >- (qexists_tac `q2l` >> rw[] >> fs[EVERY_APPEND]
-          >> metis_tac[qrel_queue_reorder,APPEND_ASSOC,EVERY_APPEND])
-      >- (rename1 `[_;_] = a1 ++ _ ++ _`
-          >> Cases_on `a1`
-          >- (fs[] >> rveq >> qexists_tac `q1++[(p1,d1)]` >> rw[qrel_refl])
-          >> fs[] >> rveq
-          >> fs[APPEND_EQ_SING |> CONV_RULE(LHS_CONV SYM_CONV)] >> rveq
-          >> qexists_tac `q1` >> rw[]
-          >> qmatch_goalsub_abbrev_tac `qrel a1 a2`
-          >> `a1 = a2` suffices_by rw[qrel_refl]
-          >> unabbrev_all_tac
-          >> rw[])
-      >- (qexists_tac `q1 ++ [(p1,d1); (p2,d2)] ++ l` >> rw[] >> fs[EVERY_APPEND]
-          >> metis_tac[qrel_queue_reorder,APPEND_ASSOC])));
-
-val qrel_cons_IMP = Q.prove(
-  `!q1 q2 qe. qrel (qe::q1) q2 ==> ?q2l q2r. q2 = q2l ++ [qe] ++ q2r /\ qrel q1 (q2l++q2r) /\ EVERY (λ(p,_). p ≠ FST qe) q2l`,
-  rpt gen_tac
-  >> `qe::q1 = [] ++ [qe] ++ q1` by rw[]
-  >> pop_assum(fn thm => PURE_ONCE_REWRITE_TAC [thm])
-  >> rpt strip_tac
-  >> dxrule qrel_cons_IMP_lemma >> rw[]);
-
-val qrel_snoc_IMP = Q.prove(
-  `!q1 q2 qe. qrel (SNOC qe q1) q2 ==> ?q2l q2r. q2 = q2l ++ [qe] ++ q2r /\ qrel q1 (q2l++q2r) /\ EVERY (λ(p,_). p ≠ FST qe) q2r`,
-  rpt gen_tac
-  >> `SNOC qe q1 = q1 ++ [qe] ++ []` by rw[SNOC_APPEND]
-  >> pop_assum(fn thm => PURE_ONCE_REWRITE_TAC [thm])
-  >> rpt strip_tac
-  >> dxrule qrel_snoc_IMP_lemma >> rw[]);
-
-val qrel_consE = Q.store_thm("qrel_consE",
-  `!q1 q2 qe. qrel (qe::q1) (qe::q2) ==> qrel q1 q2`,
-  `!qq1 qq2. qrel qq1 qq2 ==> (!q1 q2 qe. qq1 = (qe::q1) /\ qq2 = (qe::q2) ==> qrel q1 q2)`
-    suffices_by metis_tac[qrel_refl]
-  >> ho_match_mp_tac qrel_strongind >> rpt strip_tac
-  >> fs[] >> rveq
-  >- metis_tac[qrel_rules]
-  >- metis_tac[qrel_rules]
-  >- (imp_res_tac qrel_LENGTH
-      >> qpat_x_assum `qrel _ (_::_)` (assume_tac o MATCH_MP qrel_sym)
-      >> imp_res_tac qrel_cons_IMP
-      >> rveq >> fs[]
-      >> match_mp_tac qrel_trans >> asm_exists_tac >> rw[]
-      >> match_mp_tac qrel_sym
-      >> match_mp_tac qrel_trans >> asm_exists_tac >> rw[]
-      >> fs[APPEND_EQ_APPEND_MID] >> rveq >> fs[] >> rpt(pairarg_tac >> fs[])
-      >> fs[APPEND_EQ_SING |> CONV_RULE(LHS_CONV SYM_CONV)] >> rw[qrel_refl])
-  >- (Cases_on `q1` >> fs[] >> rveq
-      >> match_mp_tac qrel_queue_reorder >> rw[]));
-
-val qrel_snocE = Q.store_thm("qrel_snocE",
-  `!q1 q2 qe. qrel (SNOC qe q1) (SNOC qe q2) ==> qrel q1 q2`,
-  `!qq1 qq2. qrel qq1 qq2 ==> (!q1 q2 qe. qq1 = (SNOC qe q1) /\ qq2 = (SNOC qe q2) ==> qrel q1 q2)`
-    suffices_by metis_tac[qrel_refl]
-  >> ho_match_mp_tac qrel_strongind >> rpt strip_tac
-  >> fs[] >> rveq
-  >- metis_tac[qrel_rules]
-  >- metis_tac[qrel_rules]
-  >- (imp_res_tac qrel_LENGTH
-      >> qpat_x_assum `qrel _ (_ ++ _)` (assume_tac o MATCH_MP qrel_sym)
-      >> imp_res_tac (qrel_snoc_IMP |> REWRITE_RULE [SNOC_APPEND])
-      >> rveq >> fs[]
-      >> match_mp_tac qrel_trans >> asm_exists_tac >> rw[]
-      >> match_mp_tac qrel_sym
-      >> match_mp_tac qrel_trans >> asm_exists_tac >> rw[]
-      >> fs[APPEND_EQ_APPEND_MID] >> rveq >> fs[] >> rpt(pairarg_tac >> fs[])
-      >> fs[APPEND_EQ_SING |> CONV_RULE(LHS_CONV SYM_CONV)] >> rw[qrel_refl])
-  >- (Q.ISPEC_THEN `q2` assume_tac SNOC_CASES >> fs[] >> rveq
-      >> fs[] >> rveq
-      >> match_mp_tac qrel_queue_reorder >> rw[]));
-
-val qrel_append_r_E = Q.store_thm("qrel_append_r_E",
-  `!q3 q1 q2. qrel (q1++q3) (q2++q3) ==> qrel q1 q2`,
-  ho_match_mp_tac SNOC_INDUCT >> rpt strip_tac >> fs[APPEND_SNOC] >> metis_tac[qrel_snocE]);
-
-val qrel_append_l_E = Q.store_thm("qrel_append_l_E",
-  `!q1 q2 q3. qrel (q1++q2) (q1++q3) ==> qrel q2 q3`,
-  Induct >> rpt strip_tac >> fs[] >> metis_tac[qrel_consE]);
-
-val qcong_nil_rel_nil = Q.store_thm("qcong_nil_rel_nil",
-  `!n2.
-    qcong NNil n2
-    ==> n2 = NNil`,
-  `!n1 n2.
-    qcong n1 n2
-    ==> (n1 = NNil ==> n2 = NNil)
-        /\ (n2 = NNil ==> n1 = NNil)`
-    suffices_by metis_tac[]
-  >> ho_match_mp_tac qcong_strongind >> rpt strip_tac
-  >> rveq >> fs[]);
-
-val qcong_endpoint_rel_endpoint = Q.store_thm("qcong_endpoint_rel_endpoint",
-  `!p1 s1 e1 n2.
-    qcong (NEndpoint p1 s1 e1) n2
-    ==> ?s2. n2 = (NEndpoint p1 s2 e1)`,
-  `!n1 n2.
-    qcong n1 n2
-    ==> (!p1 s1 e1. n1 = NEndpoint p1 s1 e1 ==> ?s2. n2 = NEndpoint p1 s2 e1)
-        /\ (!p2 s2 e2. n2 = NEndpoint p2 s2 e2 ==> ?s1. n1 = NEndpoint p2 s1 e2)`
-    suffices_by metis_tac[]
-  >> ho_match_mp_tac qcong_strongind >> rpt strip_tac
-  >> rveq >> fs[])
-
-val qcong_par_rel_par = Q.store_thm("qcong_par_rel_par",
-  `!n1 n2 n3.
-    qcong (NPar n1 n2) n3
-    ==> ?n4 n5. n3 = (NPar n4 n5) /\ qcong n1 n4 /\ qcong n2 n5`,
-  `!n1 n2.
-    qcong n1 n2
-    ==> (!n3 n4. n1 = NPar n3 n4 ==> ?n5 n6. n2 = NPar n5 n6 /\ qcong n3 n5 /\ qcong n4 n6)
-        /\ (!n3 n4. n2 = NPar n3 n4 ==> ?n5 n6. n1 = NPar n5 n6 /\ qcong n5 n3 /\ qcong n6 n4)`
-    suffices_by metis_tac[]
-  >> ho_match_mp_tac qcong_strongind >> rpt strip_tac
-  >> rveq >> fs[qcong_refl,qcong_sym]
-  >> rpt(first_x_assum drule >> strip_tac) >> metis_tac[qcong_rules]);
-
-val qcong_par_rel_par_sym = Q.store_thm("qcong_par_rel_par_sym",
-  `!n1 n2 n3.
-    qcong n1 (NPar n2 n3)
-    ==> ?n4 n5. n1 = (NPar n4 n5) /\ qcong n4 n2 /\ qcong n5 n3`,
-  metis_tac[qcong_par_rel_par,qcong_sym]);
-
-val qcong_IMP_qrel = Q.store_thm("qcong_IMP_qrel",
-  `!p1 s1 e1 p2 s2 e2.
-    qcong (NEndpoint p1 s1 e1) (NEndpoint p2 s2 e2)
-    ==> qrel s1.queue s2.queue`,
-  `!n1 n2.
-    qcong n1 n2 ==>
-    !p1 s1 e1 p2 s2 e2.
-    n1 = NEndpoint p1 s1 e1 /\ n2 = NEndpoint p2 s2 e2
-    ==> qrel s1.queue s2.queue` suffices_by metis_tac[]
-  >> ho_match_mp_tac qcong_strongind >> rpt strip_tac
-  >> rveq >> fs[] >> rveq >> simp[]
-  >> metis_tac[qrel_rules,qcong_endpoint_rel_endpoint]);
-
-val qcong_bindings_eq = Q.store_thm("qcong_bindings_eq",
-  `!p1 s1 e1 p2 s2 e2.
-    qcong (NEndpoint p1 s1 e1) (NEndpoint p2 s2 e2)
-    ==> s1.bindings = s2.bindings`,
-  `!n1 n2.
-    qcong n1 n2 ==>
-    !p1 s1 e1 p2 s2 e2.
-    n1 = NEndpoint p1 s1 e1 /\ n2 = NEndpoint p2 s2 e2
-    ==> s1.bindings = s2.bindings` suffices_by metis_tac[]
-  >> ho_match_mp_tac qcong_strongind >> rpt strip_tac
-  >> rveq >> fs[] >> rveq >> simp[]
-  >> metis_tac[qrel_rules,qcong_endpoint_rel_endpoint]);
-
-val qcong_queue_reorder'' = Q.store_thm("qcong_queue_reorder''",
-  `∀p e p1 d1 p2 d2 b q1 q2.
-     p1 ≠ p2
-     ⇒ qcong (NEndpoint p (<|bindings := b; queue:=q1 ++ [(p1,d1);(p2,d2)] ++ q2|>) e)
-              (NEndpoint p (<|bindings := b; queue:= q1 ++ [(p2,d2);(p1,d1)] ++ q2|>) e)`,
-  rpt strip_tac
-  >> qmatch_goalsub_abbrev_tac `qcong (NEndpoint _ a1 _) (NEndpoint _ (<|bindings := _; queue := a2|>) _)`
-  >> `<|bindings := b; queue := a2|> = a1 with queue := a2` by(unabbrev_all_tac >> fs[])
-  >> pop_assum (fn thm => PURE_ONCE_REWRITE_TAC [thm])
-  >> unabbrev_all_tac
-  >> match_mp_tac qcong_queue_reorder
-  >> simp[]);
-
-val qcong_endpoints = Q.store_thm("qcong_endpoints",
-  `!n1 n2. qcong n1 n2 ==> MAP FST (endpoints n2) = MAP FST (endpoints n1)`,
-  ho_match_mp_tac qcong_strongind >> rw[endpoints_def])
-
 val trans_enqueue' = Q.store_thm("trans_enqueue'",
   `∀conf s d p1 p2 e q.
      p1 ≠ p2
-     ⇒ trans conf (NEndpoint p2 (s with queue := q) e) (LReceive p1 d p2)
-       (NEndpoint p2 (s with queue := SNOC (p1,d) q) e)`,
+     ⇒ trans conf (NEndpoint p2 (s with queues := q) e) (LReceive p1 d p2)
+       (NEndpoint p2 (s with queues := qpush q p1 d) e)`,
   rpt strip_tac
-  >> `s with queue := SNOC (p1,d) q = (s with queue := q) with queue := SNOC (p1,d) ((s with queue := q).queue)` by fs[]
+  >> `s with queues := qpush q p1 d = (s with queues := q) with queues := qpush ((s with queues := q).queues) p1 d` by fs[]
   >> pop_assum (fn thm => PURE_ONCE_REWRITE_TAC [thm])
   >> match_mp_tac trans_enqueue
   >> simp[]);
 
-val trans_dequeue_last_payload' = Q.store_thm("trans_dequeue_last_payload'",
-  `∀conf s v p1 p2 e q1 q2 d ds.
-     p1 ≠ p2 ∧
-     EVERY (λ(p,_). p ≠ p1) q1 ∧ final d ⇒
-     trans conf (NEndpoint p2 (s with queue := q1 ⧺ [(p1,d)] ⧺ q2) (Receive p1 v ds e)) LTau
-       (NEndpoint p2
-          <|bindings := s.bindings |+ (v,FLAT (SNOC (unpad d) ds));
-            queue := q1 ⧺ q2|> e)`,
-  rpt strip_tac
-  >> qmatch_goalsub_abbrev_tac `_ with queue := a1`
-  >> `s.bindings = (s with queue := a1).bindings` by simp[]
-  >> pop_assum (fn thm => PURE_ONCE_REWRITE_TAC [thm])
-  >> match_mp_tac (trans_dequeue_last_payload |> SIMP_RULE (srw_ss()) [])
-  >> simp[]);
+Theorem qlk_qpush[simp]:
+  qlk (qpush q p1 d) p1 = qlk q p1 ++ [d]
+Proof
+  rw[qlk_def,qpush_def,fget_def,FLOOKUP_UPDATE]  
+QED
 
-val trans_dequeue_intermediate_payload' = Q.store_thm("trans_dequeue_intermediate_payload'",
-  `∀conf s v p1 p2 e q1 q2 d ds.
-     p1 ≠ p2 ∧
-     EVERY (λ(p,_). p ≠ p1) q1 ∧ intermediate d ⇒
-     trans conf (NEndpoint p2 (s with queue := q1 ⧺ [(p1,d)] ⧺ q2) (Receive p1 v ds e)) LTau
-       (NEndpoint p2 (s with queue := q1 ⧺ q2)
-          (Receive p1 v (SNOC (unpad d) ds) e))`,
-  rpt strip_tac
-  >> qmatch_goalsub_abbrev_tac `_ with queue := a1`
-  >> `s with queue := q1 ++ q2 = ((s with queue := a1) with queue := q1 ++ q2)` by fs[]
-  >> pop_assum (fn thm => PURE_ONCE_REWRITE_TAC [thm])
-  >> unabbrev_all_tac
-  >> match_mp_tac (trans_dequeue_intermediate_payload)
-  >> simp[]);
+Theorem trans_dequeue_last_payload':
+  ∀conf s1 s2 v p1 p2 e d tl ds q.
+     p1 ≠ p2 ∧ qlk s1.queues p1 = d::tl ∧ final d ∧
+     s2.bindings = s1.bindings |+ (v,FLAT (SNOC (unpad d) ds)) ∧
+     s2.queues = s1.queues |+ (p1,tl)
+     ⇒
+     trans conf (NEndpoint p2 s1 (Receive p1 v ds e)) LTau
+       (NEndpoint p2 s2 e)
+Proof
+  rpt strip_tac >>
+  drule trans_dequeue_last_payload >>
+  rpt(disch_then drule) >>
+  fs[] >>
+  disch_then(qspecl_then [‘conf’,‘v’,‘e’,‘ds’] mp_tac) >>
+  qmatch_goalsub_abbrev_tac ‘trans _ _ _ (NEndpoint _ a1 _)’ >>
+  ‘a1 = s2’ suffices_by simp[] >>
+  rw[Abbr ‘a1’,state_component_equality]
+QED
+
+Theorem trans_dequeue_intermediate_payload':
+  ∀conf s1 s2 v p1 p2 e d ds tl.
+     p1 ≠ p2 ∧ qlk s1.queues p1 = d::tl ∧ intermediate d ∧
+     s2.bindings = s1.bindings ∧
+     s2.queues = s1.queues |+ (p1,tl)
+      ⇒
+     trans conf (NEndpoint p2 s1 (Receive p1 v ds e)) LTau
+       (NEndpoint p2 s2
+          (Receive p1 v (SNOC (unpad d) ds) e))
+Proof
+  rpt strip_tac >>
+  drule trans_dequeue_intermediate_payload >>
+  rpt(disch_then drule) >>
+  fs[] >>
+  disch_then(qspecl_then [‘conf’,‘v’,‘e’,‘ds’] mp_tac) >>
+  qmatch_goalsub_abbrev_tac ‘trans _ _ _ (NEndpoint _ a1 _)’ >>
+  ‘a1 = s2’ suffices_by simp[] >>
+  rw[Abbr ‘a1’,state_component_equality]
+QED
 
 val trans_let' = Q.store_thm("trans_let'",
   `∀conf s v p f vl e q.
          EVERY IS_SOME (MAP (FLOOKUP s.bindings) vl) ⇒
-         trans conf (NEndpoint p (s with queue:= q) (Let v f vl e)) LTau
+         trans conf (NEndpoint p (s with queues:= q) (Let v f vl e)) LTau
            (NEndpoint p
               (<|bindings := s.bindings |+ (v,f (MAP (THE ∘ FLOOKUP s.bindings) vl));
-                 queue:= q
+                 queues:= q
                  |>) e)`,
   rpt strip_tac
   >> qmatch_goalsub_abbrev_tac `trans _ (NEndpoint _ s1 _) _ (NEndpoint _ s2 _)`
@@ -502,359 +121,10 @@ val trans_let' = Q.store_thm("trans_let'",
   >> match_mp_tac trans_let
   >> simp[]);
 
-val qcong_sym_eq = Q.store_thm("qcong_sym_eq",
-`∀p q. qcong p q = qcong q p`,metis_tac[qcong_sym]);
-
 val trans_IMP_weak_trans = Q.store_thm("trans_IMP_weak_trans",
   `∀conf p alpha q. trans conf p alpha q ==> weak_trans conf p alpha q`,
   rw[weak_trans_def,weak_tau_trans_def]
   >> metis_tac[RTC_REFL,RTC_SINGLE,reduction_def]);
-
-val qcong_trans_eq = Q.store_thm("qcong_trans_eq",
-  `∀p1 q1 .
-     qcong p1 q1
-     ⇒ ∀ conf alpha p2 q2.
-            ((trans conf p1 alpha p2 ⇒ (∃q2. trans conf q1 alpha q2 ∧ qcong p2 q2))
-         ∧ (trans conf q1 alpha q2 ⇒ (∃p2. trans conf p1 alpha p2 ∧ qcong p2 q2)))`,
-  ho_match_mp_tac qcong_strongind
-  >> rpt strip_tac
-  >- metis_tac[qcong_rules]
-  >- metis_tac[qcong_rules]
-  >- metis_tac[qcong_rules]
-  >- metis_tac[qcong_rules]
-  >- metis_tac[qcong_rules]
-  >- metis_tac[qcong_rules]
-  >- (* qcong_queue_reorder *)
-     (qpat_x_assum `trans _ _ _ _` (assume_tac
-                                    o REWRITE_RULE [Once payloadSemTheory.trans_cases])
-      >> fs[] >> rveq
-      >> TRY(qmatch_goalsub_abbrev_tac `qcong (NEndpoint a1 a2 a3)`
-             >> qexists_tac `NEndpoint a1 (a2 with queue := q1 ⧺ [(p2,d2); (p1,d1)] ⧺ q2) a3`
-             >> conj_tac
-             >- (unabbrev_all_tac
-                 >> MAP_FIRST match_mp_tac (CONJUNCTS payloadSemTheory.trans_rules)
-                 >> fs[])
-             >- metis_tac[qcong_rules])
-      >> TRY(qmatch_goalsub_abbrev_tac `qcong (NEndpoint a1 (a2 with queue := SNOC a3 _) a4)`
-             >> qexists_tac `NEndpoint a1 (a2 with queue := SNOC a3 (q1 ++ [(p2,d2);(p1,d1)] ++ q2)) a4`
-             >> conj_tac
-             >- (unabbrev_all_tac
-                 >> MAP_FIRST match_mp_tac [trans_enqueue']
-                 >> simp[])
-             >- (simp[SNOC_APPEND] >> metis_tac[qcong_queue_reorder',APPEND_ASSOC]))
-      >> TRY(qmatch_goalsub_abbrev_tac `qcong (NEndpoint a1 (a2 with bindings := a3) a4)`
-              >> qexists_tac `NEndpoint a1 ((a2 with queue := (q1 ++ [(p2,d2);(p1,d1)] ++ q2))
-                                                with bindings := a3) a4`
-             >> conj_tac
-             >- (unabbrev_all_tac
-                 >> `s.bindings = (s with queue := q1 ++ [(p2,d2); (p1,d1)] ++ q2).bindings`
-                       by simp[]
-                 >> pop_assum (fn thm => PURE_ONCE_REWRITE_TAC [thm])
-                 >> match_mp_tac trans_let
-                 >> simp[])
-             >- (`(a2 with bindings := a3).queue = a2.queue` by fs[]
-                 >> PURE_ONCE_REWRITE_TAC [GSYM endpointLangTheory.state_fupdcanon]
-                 >> metis_tac [qcong_queue_reorder]))
-      >> TRY(fs[APPEND_EQ_APPEND_MID] >> rveq >> fs[Once APPEND_EQ_CONS]
-             >> fs[APPEND_EQ_SING] >> rveq >> fs[] >> rveq >> fs[]
-             >> TRY(qmatch_goalsub_abbrev_tac
-                      `qcong (NEndpoint a1 (<|bindings := a2 ; queue := a3 ++ a4 ++ [a5;a6] ++ a7|>) a8)`
-                    >> qexists_tac
-                       `NEndpoint a1 (<|bindings := a2 ; queue := a3 ++ a4 ++ [a6;a5] ++ a7|>) a8`
-                    >> conj_tac
-                    >- (unabbrev_all_tac
-                        >> SIMP_TAC bool_ss [GSYM APPEND_ASSOC]
-                        >> SIMP_TAC bool_ss [Once APPEND_ASSOC]
-                        >> match_mp_tac trans_dequeue_last_payload'
-                        >> simp[])
-                    >> metis_tac[qcong_queue_reorder''])
-             >> TRY(qmatch_goalsub_abbrev_tac
-                      `qcong (NEndpoint a1 (<|bindings := a2 ; queue := a3 ++ [a4] ++ a5|>) a6)`
-                    >> qexists_tac
-                       `NEndpoint a1 (<|bindings := a2 ; queue := a3 ++ [a4] ++ a5|>) a6`
-                    >> conj_tac
-                    >- (unabbrev_all_tac
-                        >> PURE_ONCE_REWRITE_TAC
-                           [Q.prove(`!l1 e1 l2. l1 ++ [e1] ++ l2 = l1 ++ (e1::l2)`,
-                                    simp[])]
-                        >> PURE_ONCE_REWRITE_TAC
-                           [Q.prove(`!l1 e1 e2 l2. l1 ++ [e1;e2] ++ l2 = l1 ++ [e1] ++ (e2::l2)`,
-                                    simp[])]
-                        >> match_mp_tac trans_dequeue_last_payload'
-                        >> simp[])
-                    >> metis_tac[qcong_refl])
-             >> TRY(qmatch_goalsub_abbrev_tac
-                      `qcong (NEndpoint a1 (<|bindings := a2 ; queue := a3 ++ [a4] ++ a5|>) a6)`
-                    >> qexists_tac
-                       `NEndpoint a1 (<|bindings := a2 ; queue := a3 ++ [a4] ++ a5|>) a6`
-                    >> conj_tac
-                    >- (unabbrev_all_tac
-                        >> PURE_ONCE_REWRITE_TAC
-                           [Q.prove(`!l1 e1 e2 l2. l1 ++ [e1;e2] ++ l2 = (l1 ++ [e1]) ++ [e2] ++ l2`,
-                                    simp[])]
-                        >> match_mp_tac trans_dequeue_last_payload'
-                        >> simp[])
-                    >> metis_tac[qcong_refl])
-             >> TRY(qmatch_goalsub_abbrev_tac
-                      `qcong (NEndpoint a1 (<|bindings := a2 ; queue := a3 ++ [a4;a5] ++ a6 ++ a7|>) a8)`
-                    >> qexists_tac
-                       `NEndpoint a1 (<|bindings := a2 ; queue := a3 ++ [a5;a4] ++ a6 ++ a7|>) a8`
-                    >> conj_tac
-                    >- (unabbrev_all_tac
-                        >> match_mp_tac trans_dequeue_last_payload'
-                        >> simp[])
-                    >> metis_tac[qcong_queue_reorder'',APPEND_ASSOC])
-             >> TRY(qmatch_goalsub_abbrev_tac
-                      `qcong (NEndpoint a1 (a2 with queue := a3 ++ a4 ++ [a5;a6] ++ a7) a8)`
-                    >> qexists_tac
-                       `NEndpoint a1 (a2 with queue := a3 ++ a4 ++ [a6;a5] ++ a7) a8`
-                    >> conj_tac
-                    >- (unabbrev_all_tac
-                        >> SIMP_TAC bool_ss [GSYM APPEND_ASSOC]
-                        >> SIMP_TAC bool_ss [Once APPEND_ASSOC]
-                        >> MAP_FIRST match_mp_tac
-                                     [trans_dequeue_intermediate_payload']
-                        >> simp[])
-                    >> metis_tac[qcong_queue_reorder'])
-             >> TRY(qmatch_goalsub_abbrev_tac
-                      `qcong (NEndpoint a1 (a2 with queue := a3 ++ [a4] ++ a5) a6)`
-                    >> qexists_tac
-                       `NEndpoint a1 (a2 with queue := a3 ++ [a4] ++ a5) a6`
-                    >> conj_tac
-                    >- (unabbrev_all_tac
-                        >> PURE_ONCE_REWRITE_TAC
-                           [Q.prove(`!l1 e1 l2. l1 ++ [e1] ++ l2 = l1 ++ (e1::l2)`,
-                                    simp[])]
-                        >> PURE_ONCE_REWRITE_TAC
-                           [Q.prove(`!l1 e1 e2 l2. l1 ++ [e1;e2] ++ l2 = l1 ++ [e1] ++ (e2::l2)`,
-                                    simp[])]
-                        >> MAP_FIRST match_mp_tac
-                                     [trans_dequeue_intermediate_payload']
-                        >> simp[])
-                    >> metis_tac[qcong_refl])
-             >> TRY(qmatch_goalsub_abbrev_tac
-                      `qcong (NEndpoint a1 (a2 with queue := a3 ++ [a4] ++ a5) a6)`
-                    >> qexists_tac
-                       `NEndpoint a1 (a2 with queue := a3 ++ [a4] ++ a5) a6`
-                    >> conj_tac
-                    >- (unabbrev_all_tac
-                        >> PURE_ONCE_REWRITE_TAC
-                           [Q.prove(`!l1 e1 e2 l2. l1 ++ [e1;e2] ++ l2 = (l1 ++ [e1]) ++ [e2] ++ l2`,
-                                    simp[])]
-                        >> MAP_FIRST match_mp_tac
-                                     [trans_dequeue_intermediate_payload']
-                        >> simp[])
-                    >> metis_tac[qcong_refl])
-             >> TRY(qmatch_goalsub_abbrev_tac
-                      `qcong (NEndpoint a1 (a2 with queue := a3 ++ [a4;a5] ++ a6 ++ a7) a8)`
-                    >> qexists_tac
-                       `NEndpoint a1 (a2 with queue := a3 ++ [a5;a4] ++ a6 ++ a7) a8`
-                    >> conj_tac
-                    >- (unabbrev_all_tac
-                        >> MAP_FIRST match_mp_tac
-                                     [trans_dequeue_intermediate_payload']
-                        >> simp[])
-                    >> metis_tac[qcong_queue_reorder',APPEND_ASSOC])))
-  >- (* qcong_queue_reorder, symmetric case *)
-     (qmatch_asmsub_abbrev_tac `NEndpoint _ s' _`
-      >> `s'.queue = q1 ⧺ [(p2,d2); (p1,d1)] ⧺ q2` by(unabbrev_all_tac >> simp[])
-      >> `s = s' with queue := q1 ⧺ [(p1,d1); (p2,d2)] ⧺ q2`
-            by(unabbrev_all_tac >> simp[endpointLangTheory.state_component_equality])
-      >> pop_assum (fn thm => fs[thm])
-      >> qpat_x_assum `Abbrev _` kall_tac
-      >> rename1 `s with queue := _ ++ [(p3,d3); (p4,d4)] ++ _`
-      >> rename1 `_ with queue := _ ++ [(p2,d2); (p1,d1)] ++ _`
-      >> PURE_ONCE_REWRITE_TAC [qcong_sym_eq]
-      >> qpat_x_assum `trans _ _ _ _` (assume_tac
-                                       o REWRITE_RULE [Once payloadSemTheory.trans_cases])
-      >> fs[] >> rveq
-      >> TRY(qmatch_goalsub_abbrev_tac `qcong (NEndpoint a1 a2 a3)`
-             >> qexists_tac `NEndpoint a1 (a2 with queue := q1 ⧺ [(p2,d2); (p1,d1)] ⧺ q2) a3`
-             >> conj_tac
-             >- (unabbrev_all_tac
-                 >> MAP_FIRST match_mp_tac (CONJUNCTS payloadSemTheory.trans_rules)
-                 >> fs[])
-             >- metis_tac[qcong_rules])
-      >> TRY(qmatch_goalsub_abbrev_tac `qcong (NEndpoint a1 (a2 with queue := SNOC a3 _) a4)`
-             >> qexists_tac `NEndpoint a1 (a2 with queue := SNOC a3 (q1 ++ [(p2,d2);(p1,d1)] ++ q2)) a4`
-             >> conj_tac
-             >- (unabbrev_all_tac
-                 >> MAP_FIRST match_mp_tac [trans_enqueue']
-                 >> simp[])
-             >- (simp[SNOC_APPEND] >> metis_tac[qcong_queue_reorder',APPEND_ASSOC]))
-      >> TRY(qmatch_goalsub_abbrev_tac `qcong (NEndpoint a1 (a2 with bindings := a3) a4)`
-              >> qexists_tac `NEndpoint a1 ((a2 with queue := (q1 ++ [(p2,d2);(p1,d1)] ++ q2))
-                                                with bindings := a3) a4`
-             >> conj_tac
-             >- (unabbrev_all_tac
-                 >> `s.bindings = (s with queue := q1 ++ [(p2,d2); (p1,d1)] ++ q2).bindings`
-                       by simp[]
-                 >> pop_assum (fn thm => PURE_ONCE_REWRITE_TAC [thm])
-                 >> match_mp_tac trans_let
-                 >> simp[])
-             >- (`(a2 with bindings := a3).queue = a2.queue` by fs[]
-                 >> PURE_ONCE_REWRITE_TAC [GSYM endpointLangTheory.state_fupdcanon]
-                 >> metis_tac [qcong_queue_reorder]))
-      >> TRY(fs[APPEND_EQ_APPEND_MID] >> rveq >> fs[Once APPEND_EQ_CONS]
-             >> fs[APPEND_EQ_SING] >> rveq >> fs[] >> rveq >> fs[]
-             >> TRY(qmatch_goalsub_abbrev_tac
-                      `qcong (NEndpoint a1 (<|bindings := a2 ; queue := a3 ++ a4 ++ [a5;a6] ++ a7|>) a8)`
-                    >> qexists_tac
-                       `NEndpoint a1 (<|bindings := a2 ; queue := a3 ++ a4 ++ [a6;a5] ++ a7|>) a8`
-                    >> conj_tac
-                    >- (unabbrev_all_tac
-                        >> SIMP_TAC bool_ss [GSYM APPEND_ASSOC]
-                        >> SIMP_TAC bool_ss [Once APPEND_ASSOC]
-                        >> match_mp_tac trans_dequeue_last_payload'
-                        >> simp[])
-                    >> metis_tac[qcong_queue_reorder''])
-             >> TRY(qmatch_goalsub_abbrev_tac
-                      `qcong (NEndpoint a1 (<|bindings := a2 ; queue := a3 ++ [a4] ++ a5|>) a6)`
-                    >> qexists_tac
-                       `NEndpoint a1 (<|bindings := a2 ; queue := a3 ++ [a4] ++ a5|>) a6`
-                    >> conj_tac
-                    >- (unabbrev_all_tac
-                        >> PURE_ONCE_REWRITE_TAC
-                           [Q.prove(`!l1 e1 l2. l1 ++ [e1] ++ l2 = l1 ++ (e1::l2)`,
-                                    simp[])]
-                        >> PURE_ONCE_REWRITE_TAC
-                           [Q.prove(`!l1 e1 e2 l2. l1 ++ [e1;e2] ++ l2 = l1 ++ [e1] ++ (e2::l2)`,
-                                    simp[])]
-                        >> match_mp_tac trans_dequeue_last_payload'
-                        >> simp[])
-                    >> metis_tac[qcong_refl])
-             >> TRY(qmatch_goalsub_abbrev_tac
-                      `qcong (NEndpoint a1 (<|bindings := a2 ; queue := a3 ++ [a4] ++ a5|>) a6)`
-                    >> qexists_tac
-                       `NEndpoint a1 (<|bindings := a2 ; queue := a3 ++ [a4] ++ a5|>) a6`
-                    >> conj_tac
-                    >- (unabbrev_all_tac
-                        >> PURE_ONCE_REWRITE_TAC
-                           [Q.prove(`!l1 e1 e2 l2. l1 ++ [e1;e2] ++ l2 = (l1 ++ [e1]) ++ [e2] ++ l2`,
-                                    simp[])]
-                        >> match_mp_tac trans_dequeue_last_payload'
-                        >> simp[])
-                    >> metis_tac[qcong_refl])
-             >> TRY(qmatch_goalsub_abbrev_tac
-                      `qcong (NEndpoint a1 (<|bindings := a2 ; queue := a3 ++ [a4;a5] ++ a6 ++ a7|>) a8)`
-                    >> qexists_tac
-                       `NEndpoint a1 (<|bindings := a2 ; queue := a3 ++ [a5;a4] ++ a6 ++ a7|>) a8`
-                    >> conj_tac
-                    >- (unabbrev_all_tac
-                        >> match_mp_tac trans_dequeue_last_payload'
-                        >> simp[])
-                    >> metis_tac[qcong_queue_reorder'',APPEND_ASSOC])
-             >> TRY(qmatch_goalsub_abbrev_tac
-                      `qcong (NEndpoint a1 (a2 with queue := a3 ++ a4 ++ [a5;a6] ++ a7) a8)`
-                    >> qexists_tac
-                       `NEndpoint a1 (a2 with queue := a3 ++ a4 ++ [a6;a5] ++ a7) a8`
-                    >> conj_tac
-                    >- (unabbrev_all_tac
-                        >> SIMP_TAC bool_ss [GSYM APPEND_ASSOC]
-                        >> SIMP_TAC bool_ss [Once APPEND_ASSOC]
-                        >> MAP_FIRST match_mp_tac
-                                     [trans_dequeue_intermediate_payload']
-                        >> simp[])
-                    >> metis_tac[qcong_queue_reorder'])
-             >> TRY(qmatch_goalsub_abbrev_tac
-                      `qcong (NEndpoint a1 (a2 with queue := a3 ++ [a4] ++ a5) a6)`
-                    >> qexists_tac
-                       `NEndpoint a1 (a2 with queue := a3 ++ [a4] ++ a5) a6`
-                    >> conj_tac
-                    >- (unabbrev_all_tac
-                        >> PURE_ONCE_REWRITE_TAC
-                           [Q.prove(`!l1 e1 l2. l1 ++ [e1] ++ l2 = l1 ++ (e1::l2)`,
-                                    simp[])]
-                        >> PURE_ONCE_REWRITE_TAC
-                           [Q.prove(`!l1 e1 e2 l2. l1 ++ [e1;e2] ++ l2 = l1 ++ [e1] ++ (e2::l2)`,
-                                    simp[])]
-                        >> MAP_FIRST match_mp_tac
-                                     [trans_dequeue_intermediate_payload']
-                        >> simp[])
-                    >> metis_tac[qcong_refl])
-             >> TRY(qmatch_goalsub_abbrev_tac
-                      `qcong (NEndpoint a1 (a2 with queue := a3 ++ [a4] ++ a5) a6)`
-                    >> qexists_tac
-                       `NEndpoint a1 (a2 with queue := a3 ++ [a4] ++ a5) a6`
-                    >> conj_tac
-                    >- (unabbrev_all_tac
-                        >> PURE_ONCE_REWRITE_TAC
-                           [Q.prove(`!l1 e1 e2 l2. l1 ++ [e1;e2] ++ l2 = (l1 ++ [e1]) ++ [e2] ++ l2`,
-                                    simp[])]
-                        >> MAP_FIRST match_mp_tac
-                                     [trans_dequeue_intermediate_payload']
-                        >> simp[])
-                    >> metis_tac[qcong_refl])
-             >> TRY(qmatch_goalsub_abbrev_tac
-                      `qcong (NEndpoint a1 (a2 with queue := a3 ++ [a4;a5] ++ a6 ++ a7) a8)`
-                    >> qexists_tac
-                       `NEndpoint a1 (a2 with queue := a3 ++ [a5;a4] ++ a6 ++ a7) a8`
-                    >> conj_tac
-                    >- (unabbrev_all_tac
-                        >> MAP_FIRST match_mp_tac
-                                     [trans_dequeue_intermediate_payload']
-                        >> simp[])
-                    >> metis_tac[qcong_queue_reorder',APPEND_ASSOC])))
-  >- (qpat_x_assum `trans _ (NPar _ _) _ _` (assume_tac
-                                             o REWRITE_RULE [Once payloadSemTheory.trans_cases])
-      >> fs[] >> rveq
-      >> EVERY_ASSUM imp_res_tac
-      >> imp_res_tac trans_com_l
-      >> imp_res_tac trans_com_r
-      >> imp_res_tac trans_par_l
-      >> imp_res_tac trans_par_r
-      >> metis_tac[qcong_rules])
-  >- (qpat_x_assum `trans _ (NPar _ _) _ _` (assume_tac
-                                             o REWRITE_RULE [Once payloadSemTheory.trans_cases])
-      >> fs[] >> rveq
-      >> EVERY_ASSUM imp_res_tac
-      >> imp_res_tac trans_com_l
-      >> imp_res_tac trans_com_r
-      >> imp_res_tac trans_par_l
-      >> imp_res_tac trans_par_r
-      >> metis_tac[qcong_rules]));
-
-val qcong_reduction_eq = Q.store_thm("qcong_reduction_eq",
-  `∀p1 q1 .
-     qcong p1 q1
-     ⇒ ∀ conf p2 q2.
-            (((reduction conf)^* p1 p2 ⇒ (∃q2. (reduction conf)^* q1 q2 ∧ qcong p2 q2))
-         ∧ ((reduction conf)^* q1 q2 ⇒ (∃p2. (reduction conf)^* p1 p2 ∧ qcong p2 q2)))`,
-  rw []
-  >- (last_x_assum mp_tac
-      \\ MAP_EVERY (W(curry Q.SPEC_TAC)) [‘q1’]
-      \\ last_x_assum mp_tac
-      \\ MAP_EVERY (W(curry Q.SPEC_TAC)) [‘p2’,‘p1’]
-      \\ ho_match_mp_tac RTC_ind \\ rw []
-      >- (qexists_tac ‘q1’ \\ fs [qcong_rules])
-      \\ fs [reduction_def]
-      \\ drule_then (qspecl_then [‘conf’,‘LTau’,‘p1'’,‘q1'’] assume_tac) qcong_trans_eq
-      \\ rfs [] \\ first_x_assum drule \\ rw [] \\ qexists_tac ‘q2'’ \\ rw []
-      \\ rw [reduction_def] \\ irule RTC_TRANS \\ qexists_tac ‘q2’  \\  rw []
-      \\ rw [reduction_def])
-  \\ last_x_assum mp_tac
-  \\ MAP_EVERY (W(curry Q.SPEC_TAC)) [‘p1’]
-  \\ last_x_assum mp_tac
-  \\ MAP_EVERY (W(curry Q.SPEC_TAC)) [‘q2’,‘q1’]
-  \\ ho_match_mp_tac RTC_ind \\ rw []
-  >- (qexists_tac ‘p1’ \\ fs [qcong_rules])
-  \\ fs [reduction_def]
-  \\ drule_then (qspecl_then [‘conf’,‘LTau’,‘p1'’,‘q1'’] assume_tac) qcong_trans_eq
-  \\ rfs [] \\ first_x_assum drule \\ rw [] \\ qexists_tac ‘p2'’ \\ rw []
-  \\ rw [reduction_def] \\ irule RTC_TRANS \\ qexists_tac ‘p2’  \\  rw []
-  \\ rw [reduction_def]);
-
-val qcong_trans_pres = Q.store_thm("qcong_trans_pres",
-  `∀p1 q1 conf alpha p2.
-     qcong p1 q1 ∧ trans conf p1 alpha p2
-     ⇒ ∃q2. trans conf q1 alpha q2 ∧ qcong p2 q2`,
-  metis_tac[qcong_trans_eq])
-
-val qcong_reduction_pres = Q.store_thm("qcong_reduction_pres",
-  `∀p1 q1 conf p2.
-     qcong p1 q1 ∧ (reduction conf)^* p1 p2
-     ⇒ ∃q2. (reduction conf)^* q1 q2 ∧ qcong p2 q2`,
-  metis_tac[qcong_reduction_eq])
 
 val reduction_par_l = Q.store_thm("reduction_par_l",
   `∀p q r conf. (reduction conf)^* p q ==> (reduction conf)^* (NPar p r) (NPar q r)`,
@@ -994,7 +264,7 @@ val receiver_is_endpoint = Q.store_thm("receiver_is_endpoint",
 val add_queue_def = Define `
   (add_queue p1 qe p2 payloadLang$NNil = NNil)
   ∧ (add_queue p1 qe p2 (NEndpoint p s e) =
-      if p1 = p then NEndpoint p (s with queue := SNOC (p2,qe) s.queue) e
+      if p1 = p then NEndpoint p (s with queues := qpush s.queues p2 qe) e
       else NEndpoint p s e
      )
   ∧ (add_queue p1 qe p2 (NPar n1 n2) = NPar (add_queue p1 qe p2 n1) (add_queue p1 qe p2 n2))
@@ -1042,13 +312,29 @@ Proof
   >> metis_tac[receiver_is_endpoint]
 QED
 
+Theorem qpush_ineq[simp]:
+  q ≠ qpush q p d
+Proof
+  rw[qpush_def,fmap_eq_flookup,FLOOKUP_UPDATE] >>
+  qexists_tac ‘p’ >> rw[qlk_def,fget_def] >>
+  TOP_CASE_TAC >> rw[]
+QED
+
+Theorem qpush_cong1[simp]:
+  qpush q p1 d = qpush q p1' d' ⇔ p1 = p1' ∧ d = d'
+Proof
+  rw[qpush_def,fmap_eq_flookup,FLOOKUP_UPDATE,EQ_IMP_THM] >>
+  pop_assum(qspec_then ‘p1’ mp_tac) >> rw[qlk_def,fget_def] >>
+  FULL_CASE_TAC >> fs[]
+QED
+        
 Theorem trans_no_selfloop:
   !conf p1 alpha p2.
   trans conf p1 alpha p2 /\ conf.payload_size > 0
   ==> p1 <> p2
 Proof
   PURE_REWRITE_TAC[GSYM AND_IMP_INTRO] >>
-  ho_match_mp_tac trans_ind >> rw[] >> fs[endpointLangTheory.state_component_equality] >>
+  ho_match_mp_tac trans_ind >> rw[] >> fs[payloadLangTheory.state_component_equality] >>
   TRY(disj2_tac) >> spose_not_then strip_assume_tac >>
   qmatch_asmsub_abbrev_tac `a1 = a2` >>
   `endpoint_size a1 = endpoint_size a2` by simp[] >>
@@ -1097,7 +383,7 @@ Proof
   >> fs[] >> rveq
   >> qhdtm_x_assum `trans` (assume_tac o SIMP_RULE std_ss [Once trans_cases])
   >> fs[] >> rveq >> fs[] >> rveq >> fs[endpoints_def,ALL_DISTINCT_APPEND]
-  >> fs[endpointLangTheory.state_component_equality]
+  >> fs[payloadLangTheory.state_component_equality]
   >> metis_tac[sender_is_endpoint,trans_no_selfloop]
 QED
 
@@ -1114,13 +400,13 @@ Proof
   fs[] >> rveq
   >- (* Send-last-payload *)
      (qhdtm_x_assum `trans` (assume_tac o SIMP_RULE std_ss [Once trans_cases]) >>
-      fs[] >> rveq >> fs[] >> rveq >> fs[endpointLangTheory.state_component_equality])
+      fs[] >> rveq >> fs[] >> rveq >> fs[payloadLangTheory.state_component_equality])
   >- (* Send-intermediate-payload *)
      (qhdtm_x_assum `trans` (assume_tac o SIMP_RULE std_ss [Once trans_cases]) >>
-      fs[] >> rveq >> fs[] >> rveq >> fs[endpointLangTheory.state_component_equality])
+      fs[] >> rveq >> fs[] >> rveq >> fs[payloadLangTheory.state_component_equality])
   >- (* Enqueue *)
      (qhdtm_x_assum `trans` (assume_tac o SIMP_RULE std_ss [Once trans_cases]) >>
-      fs[] >> rveq >> fs[] >> rveq >> fs[endpointLangTheory.state_component_equality] >>
+      fs[] >> rveq >> fs[] >> rveq >> fs[payloadLangTheory.state_component_equality] >>
       qmatch_asmsub_abbrev_tac `a1:endpoint = a2` >>
       `endpoint_size a1 = endpoint_size a2` by simp[] >>
       unabbrev_all_tac >> pop_assum mp_tac >> rpt(pop_assum kall_tac) >>
@@ -1135,27 +421,27 @@ Proof
       Cases_on `beta` >> fs[] >> metis_tac[trans_no_selfloop])
   >- (* Dequeue-last-payload *)
      (qhdtm_x_assum `trans` (assume_tac o SIMP_RULE std_ss [Once trans_cases]) >>
-      fs[] >> rveq >> fs[] >> rveq >> fs[endpointLangTheory.state_component_equality] >>
+      fs[] >> rveq >> fs[] >> rveq >> fs[payloadLangTheory.state_component_equality] >>
       qmatch_asmsub_abbrev_tac `a1:endpoint = a2` >>
       `endpoint_size a1 = endpoint_size a2` by simp[] >>
       unabbrev_all_tac >> pop_assum mp_tac >> rpt(pop_assum kall_tac) >>
       simp[endpoint_size_def])
   >- (* Dequeue-intermediate-payload *)
      (qhdtm_x_assum `trans` (assume_tac o SIMP_RULE std_ss [Once trans_cases]) >>
-      fs[] >> rveq >> fs[] >> rveq >> fs[endpointLangTheory.state_component_equality] >>
+      fs[] >> rveq >> fs[] >> rveq >> fs[payloadLangTheory.state_component_equality] >>
       qmatch_asmsub_abbrev_tac `a1:endpoint = a2` >>
       `endpoint_size a1 = endpoint_size a2` by simp[] >>
       unabbrev_all_tac >> pop_assum mp_tac >> rpt(pop_assum kall_tac) >>
       simp[endpoint_size_def])
   >- (* If-L *)
      (qhdtm_x_assum `trans` (assume_tac o SIMP_RULE std_ss [Once trans_cases]) >>
-      fs[] >> rveq >> fs[] >> rveq >> fs[endpointLangTheory.state_component_equality])
+      fs[] >> rveq >> fs[] >> rveq >> fs[payloadLangTheory.state_component_equality])
   >- (* If-R *)
      (qhdtm_x_assum `trans` (assume_tac o SIMP_RULE std_ss [Once trans_cases]) >>
-      fs[] >> rveq >> fs[] >> rveq >> fs[endpointLangTheory.state_component_equality])
+      fs[] >> rveq >> fs[] >> rveq >> fs[payloadLangTheory.state_component_equality])
   >- (* Let *)
      (qhdtm_x_assum `trans` (assume_tac o SIMP_RULE std_ss [Once trans_cases]) >>
-      fs[] >> rveq >> fs[] >> rveq >> fs[endpointLangTheory.state_component_equality])
+      fs[] >> rveq >> fs[] >> rveq >> fs[payloadLangTheory.state_component_equality])
   >- (* Par-L *)
      (qhdtm_x_assum `trans` (assume_tac o SIMP_RULE std_ss [Once trans_cases]) >>
       fs[] >> rveq >> fs[] >> rveq >> fs[] >> metis_tac[trans_no_selfloop])
@@ -1168,16 +454,6 @@ Theorem intermediate_final_IMP:
   !d. intermediate d /\ final d ==> F
 Proof
   Cases >> rpt strip_tac >> fs[intermediate_def,final_def] >> rveq >> fs[]
-QED
-
-Theorem qcong_list_trans_pres:
-  !conf p l q p'. list_trans conf p l q /\ qcong p p'
-  ==> ?q'. list_trans conf p' l q' /\ qcong q q'
-Proof
-  Induct_on `l` >>
-  rw[list_trans_def] >> simp[] >>
-  dxrule_all_then strip_assume_tac qcong_trans_pres >>
-  metis_tac[]
 QED
 
 val _ = export_theory ();
